before: frama rule

NuBasicAbstractors.thy
@@ -4,6 +4,7 @@ theory NuBasicAbstractors
 begin
 
 \<nu>overloads singular and plural
+\<nu>overloads split_cast
 
 text \<open>Basic \<nu>-abstractors\<close>
 
@@ -25,36 +26,6 @@ val th2 = SOLVED' (Tactical.REPEAT o Tactic.ares_tac @{context} @{thms \<nu>shar
 section \<open>Abstractors for specification\<close>
 
 
-subsubsection \<open>Operator Some\<close>
-(*
-definition NuSome :: " ('a :: lrep, 'b) \<nu> \<Rightarrow> ('a :: lrep, 'b set) \<nu> " ("<some>")
-  where "NuSome N h p S = (\<exists>x. x \<in> S \<and> ([h] p \<nuLinkL> N \<nuLinkR> x))"
-notation NuSome ("\<^bold>s\<^bold>o\<^bold>m\<^bold>e")
-
-lemma [simp]: "[h] p \<nuLinkL> \<^bold>s\<^bold>o\<^bold>m\<^bold>e N \<nuLinkR> X \<longleftrightarrow> (\<exists>x. x \<in> X \<and> ([h] p \<nuLinkL> N \<nuLinkR> x))" unfolding NuSome_def Refining_def Nu_def by auto
-lemma [elim,\<nu>elim]: "[h] X \<ratio> ( \<^bold>s\<^bold>o\<^bold>m\<^bold>e N) \<Longrightarrow> (\<And>x. x \<in> X \<Longrightarrow> [h] x \<ratio> N \<Longrightarrow> C) \<Longrightarrow> C" unfolding Inhabited_def by auto
-lemma [\<nu>intro]: "\<^bold>p\<^bold>r\<^bold>e\<^bold>m\<^bold>i\<^bold>s\<^bold>e X \<subseteq> X' \<Longrightarrow> [h] \<^bold>c\<^bold>a\<^bold>s\<^bold>t X \<tycolon> (\<^bold>s\<^bold>o\<^bold>m\<^bold>e N) \<longmapsto> X' \<tycolon> (\<^bold>s\<^bold>o\<^bold>m\<^bold>e N)" unfolding Cast_def by (auto 2 3)
-lemma [\<nu>intro]: "[h] \<^bold>c\<^bold>a\<^bold>s\<^bold>t x \<tycolon> N \<longmapsto> y \<tycolon> M \<^bold>w\<^bold>i\<^bold>t\<^bold>h P \<Longrightarrow> \<^bold>p\<^bold>r\<^bold>e\<^bold>m\<^bold>i\<^bold>s\<^bold>e y \<in> Y \<Longrightarrow> [h] \<^bold>c\<^bold>a\<^bold>s\<^bold>t x \<tycolon> N \<longmapsto> Y \<tycolon> (\<^bold>s\<^bold>o\<^bold>m\<^bold>e M) \<^bold>w\<^bold>i\<^bold>t\<^bold>h P" unfolding Cast_def by auto
-lemma someI_\<nu>cast: "\<^bold>p\<^bold>a\<^bold>r\<^bold>a\<^bold>m X \<Longrightarrow> \<^bold>p\<^bold>r\<^bold>e\<^bold>m\<^bold>i\<^bold>s\<^bold>e x \<in> X \<Longrightarrow> [h] \<^bold>c\<^bold>a\<^bold>s\<^bold>t x \<tycolon> N \<longmapsto> X \<tycolon> (\<^bold>s\<^bold>o\<^bold>m\<^bold>e N)" unfolding Cast_def by auto
-lemma someE_\<nu>cast[\<nu>cast_overload E]: "[h] \<^bold>c\<^bold>a\<^bold>s\<^bold>t X \<tycolon> (\<^bold>s\<^bold>o\<^bold>m\<^bold>e N) \<longmapsto> (\<exists>*some. \<tort_lbrace>some \<tycolon> N \<tort_rbrace> \<addition> (some \<in> X))" unfolding Cast_def by auto
-
-subsubsection \<open>AutoSome and AutoExTy\<close>
-
-definition SchemaSome :: " ('a :: lrep, 'b) \<nu> \<Rightarrow> ('a :: lrep, 'b set) \<nu> " ("<some''>") where "SchemaSome = NuSome"
-
-lemma [\<nu>intro]: "\<^bold>c\<^bold>a\<^bold>s\<^bold>t x \<tycolon> N \<longmapsto> y \<tycolon> \<^bold>s\<^bold>o\<^bold>m\<^bold>e M \<^bold>w\<^bold>i\<^bold>t\<^bold>h P \<Longrightarrow> \<^bold>c\<^bold>a\<^bold>s\<^bold>t x \<tycolon> N \<longmapsto> y \<tycolon> <some'> M \<^bold>w\<^bold>i\<^bold>t\<^bold>h P"
-  unfolding SchemaSome_def .
-lemma [simp]: "\<tort_lbrace> s \<tycolon> <some'> N \<tort_rbrace> = (\<exists>* x. \<tort_lbrace> x \<tycolon> N \<tort_rbrace> \<addition> (x \<in> s))" unfolding SchemaSome_def by (rule ext) auto
-
-
-lemma
-  assumes A: "\<^bold>c\<^bold>u\<^bold>r\<^bold>r\<^bold>e\<^bold>n\<^bold>t blk \<^bold>r\<^bold>e\<^bold>s\<^bold>u\<^bold>l\<^bold>t\<^bold>s \<^bold>i\<^bold>n (R\<heavy_comma> s \<tycolon> <some'> N)"
-  shows SchemaSome_ex: "\<exists>x. \<^bold>c\<^bold>u\<^bold>r\<^bold>r\<^bold>e\<^bold>n\<^bold>t blk \<^bold>r\<^bold>e\<^bold>s\<^bold>u\<^bold>l\<^bold>t\<^bold>s \<^bold>i\<^bold>n (R\<heavy_comma> x \<tycolon> N) \<addition> (x \<in> s)"
-proof -
-  have t1: "\<tort_lbrace> s \<tycolon> <some'> N \<tort_rbrace> = (\<exists>*x. \<tort_lbrace> x \<tycolon> N \<tort_rbrace> \<addition> (x \<in> s))" unfolding SchemaSome_def by (rule ext) auto
-  show ?thesis using A[simplified t1, simplified, simplified ExTyp_strip] .
-qed
-*)
 subsection \<open>\<nu>-abstraction : DeepModel\<close>
 
 definition DeepModel :: "('a::lrep, 'b) \<nu> \<Rightarrow> (deep_model, 'b) \<nu>"
@@ -106,6 +77,18 @@ lemma [\<nu>intro 30]:
   apply (cases a) apply (auto simp add: pred_option_def Ball_def nu_exps)
   by (metis MemAddrState_add_I1 MemAddrState_add_I2 nth_list_update option.sel)
 
+lemma split_cast_Array'_\<nu>app[\<nu>overload split_cast]:
+  "\<^bold>p\<^bold>a\<^bold>r\<^bold>a\<^bold>m n \<Longrightarrow> \<^bold>p\<^bold>r\<^bold>e\<^bold>m\<^bold>i\<^bold>s\<^bold>e n < length l \<Longrightarrow>
+  \<^bold>c\<^bold>a\<^bold>s\<^bold>t a \<R_arr_tail> l \<tycolon> Array' T \<longmapsto> a \<R_arr_tail> take n l \<tycolon> Array' T \<heavy_asterisk> (a ||+ n) \<R_arr_tail> drop n l \<tycolon> Array' T"
+  unfolding Cast_def Premise_def Heap_Delimiter_def apply (cases a) apply (auto simp add: nu_exps min_absorb2) 
+  subgoal for base ofs v
+    apply (rule heap_split_by_set[of _ _ "{ MemAddress (base |+ ofs + i) | i. i < n}"])
+    apply (auto simp add: pred_option_def Ball_def split: option.split)
+    apply (rule MemAddrState_restrict_I2)
+     apply (metis add.assoc add.commute less_diff_conv)
+    by simp
+  done
+
 (* lemma Array'_dual_Ref_\<nu>proc [\<nu>intro]:
  "\<^bold>p\<^bold>r\<^bold>e\<^bold>m\<^bold>i\<^bold>s\<^bold>e i < length xs \<Longrightarrow> \<^bold>p\<^bold>r\<^bold>e\<^bold>m\<^bold>i\<^bold>s\<^bold>e (xs ! i) \<noteq> None \<Longrightarrow>
   \<^bold>c\<^bold>a\<^bold>s\<^bold>t a \<R_arr_tail> xs \<tycolon> Array' N \<longmapsto> a \<R_arr_tail> xs[i := None] \<tycolon> Array' N \<heavy_asterisk> \<medium_left_bracket> (a ||+ i) \<R_arr_tail> the (xs ! i) \<tycolon> Ref N \<medium_right_bracket>
@@ -121,6 +104,8 @@ subsection \<open>\<nu>-abstraction : Array\<close>
 definition Array :: "('a::field, 'b) \<nu> \<Rightarrow> (heap, nat memaddr \<R_arr_tail> 'b list) \<nu>"
   where "Array N = Array' N <down-lift> (map_object id (map Some)) "
 
+lemma Array_to_Array': "\<tort_lbrace>a \<R_arr_tail> l \<tycolon> Array T\<tort_rbrace> = \<tort_lbrace> a \<R_arr_tail> map Some l \<tycolon> Array' T \<tort_rbrace>"
+  unfolding Array_def by auto
 (* lemma [simp]: "heap \<nuLinkL> Array N \<nuLinkR> (base |+ ofs) \<R_arr_tail> xs \<longleftrightarrow>
     (ofs + length xs \<le> segment_len base \<and>
     segment_llty base = LLTY('a) \<and>
@@ -154,8 +139,16 @@ lemma [\<nu>intro 10]: "\<^bold>d\<^bold>e\<^bold>s\<^bold>t \<^bold>c\<^bold>a\
 
 lemma [\<nu>intro]: "\<^bold>c\<^bold>a\<^bold>s\<^bold>t a \<R_arr_tail> [x] \<tycolon> Array T \<longmapsto> a \<R_arr_tail> x \<tycolon> Ref T"
   unfolding Cast_def Array_def by (cases a) (simp add: pred_option_def Ball_def)
-lemma [\<nu>intro]: "\<^bold>c\<^bold>a\<^bold>s\<^bold>t a \<R_arr_tail> x \<tycolon> Ref T \<longmapsto> a \<R_arr_tail> [x] \<tycolon> Array T"
-  unfolding Cast_def Array_def by (cases a) (auto simp add: pred_option_def Ball_def)
+
+lemma [\<nu>overload split_cast]:
+  "\<^bold>p\<^bold>a\<^bold>r\<^bold>a\<^bold>m n \<Longrightarrow> \<^bold>p\<^bold>r\<^bold>e\<^bold>m\<^bold>i\<^bold>s\<^bold>e n < length l \<Longrightarrow>
+  \<^bold>c\<^bold>a\<^bold>s\<^bold>t a \<R_arr_tail> l \<tycolon> Array T \<longmapsto> a \<R_arr_tail> take n l \<tycolon> Array T \<heavy_asterisk> (a ||+ n) \<R_arr_tail> drop n l \<tycolon> Array T"
+  by (simp add: Array_to_Array'
+      split_cast_Array'_\<nu>app[of n "map Some l" a T, simplified, simplified take_map drop_map])
+
+
+(* lemma [\<nu>intro]: "\<^bold>c\<^bold>a\<^bold>s\<^bold>t a \<R_arr_tail> x \<tycolon> Ref T \<longmapsto> a \<R_arr_tail> [x] \<tycolon> Array T"
+  unfolding Cast_def Array_def by (cases a) (auto simp add: pred_option_def Ball_def) *)
 
 (* lemma [THEN cast_dual_trans, \<nu>intro]: 
   "\<^bold>c\<^bold>a\<^bold>s\<^bold>t a \<R_arr_tail> xs \<tycolon> Array N \<longmapsto> a \<R_arr_tail> mapSome xs \<tycolon> Array' N
