NuSys.thy
@@ -229,7 +229,8 @@ lemma [\<nu>intro 10]: "\<^bold>c\<^bold>a\<^bold>s\<^bold>t A \<longmapsto> A' 
 lemma CastI[intro]: "Inhabited A \<Longrightarrow> A \<subseteq> B \<Longrightarrow> P \<Longrightarrow> \<^bold>c\<^bold>a\<^bold>s\<^bold>t A \<longmapsto> B \<^bold>w\<^bold>i\<^bold>t\<^bold>h P"
   and [intro]: "\<not> Inhabited A \<Longrightarrow> \<^bold>c\<^bold>a\<^bold>s\<^bold>t A \<longmapsto> B \<^bold>w\<^bold>i\<^bold>t\<^bold>h P" unfolding Cast_def Inhabited_def by auto *)
 
-lemma as_\<nu>proc: "\<^bold>p\<^bold>a\<^bold>r\<^bold>a\<^bold>m x' \<Longrightarrow> \<^bold>p\<^bold>r\<^bold>e\<^bold>m\<^bold>i\<^bold>s\<^bold>e x = x' \<Longrightarrow> \<^bold>c\<^bold>a\<^bold>s\<^bold>t x \<tycolon> N \<longmapsto> x' \<tycolon> N" unfolding Cast_def by auto
+lemma ie_\<nu>app: "\<^bold>p\<^bold>a\<^bold>r\<^bold>a\<^bold>m x' \<Longrightarrow> \<^bold>p\<^bold>r\<^bold>e\<^bold>m\<^bold>i\<^bold>s\<^bold>e x = x' \<Longrightarrow> \<^bold>c\<^bold>a\<^bold>s\<^bold>t x \<tycolon> N \<longmapsto> x' \<tycolon> N" unfolding Cast_def by auto
+lemma as_\<nu>app: "\<^bold>p\<^bold>a\<^bold>r\<^bold>a\<^bold>m X' \<Longrightarrow> \<^bold>c\<^bold>a\<^bold>s\<^bold>t x \<tycolon> N \<longmapsto> \<tort_lbrace>X'\<tort_rbrace> \<Longrightarrow> \<^bold>c\<^bold>a\<^bold>s\<^bold>t x \<tycolon> N \<longmapsto> \<tort_lbrace>X'\<tort_rbrace>" .
 lemma [\<nu>intro 300]: "\<^bold>p\<^bold>r\<^bold>e\<^bold>m\<^bold>i\<^bold>s\<^bold>e x = x' \<Longrightarrow> \<^bold>c\<^bold>a\<^bold>s\<^bold>t x \<tycolon> N \<longmapsto> x' \<tycolon> N" unfolding Cast_def Premise_def by simp
 lemma [\<nu>intro 2000]: "\<^bold>p\<^bold>r\<^bold>e\<^bold>m\<^bold>i\<^bold>s\<^bold>e x = x" unfolding Premise_def by simp
 
@@ -266,6 +267,10 @@ subsubsection \<open>Auto tag\<close>
 definition Auto :: " 'a \<Rightarrow> 'a " where "Auto x = x"
 
 lemma [\<nu>intro]: "\<^bold>i\<^bold>n\<^bold>t\<^bold>r\<^bold>o \<^bold>c\<^bold>a\<^bold>s\<^bold>t x \<tycolon> T \<longmapsto> x \<tycolon> Auto T" unfolding Auto_def Intro_def using cast_id .
+
+lemma Auto_cong: "\<tort_lbrace>x \<tycolon> T\<tort_rbrace> \<equiv> \<tort_lbrace>x' \<tycolon> T'\<tort_rbrace> \<Longrightarrow> \<tort_lbrace>x \<tycolon> Auto T\<tort_rbrace> \<equiv> \<tort_lbrace>x' \<tycolon> Auto T'\<tort_rbrace>" unfolding atomize_eq Auto_def .
+simproc_setup Auto_cong ("\<tort_lbrace>x \<tycolon> Auto T\<tort_rbrace>") = \<open>K (NuSimpCong.simproc @{thm Auto_cong})\<close>
+
 
 subsubsection \<open>Argument tag\<close>
 
@@ -395,6 +400,9 @@ consts Heap_Delimiter_sugar :: " 'just \<Rightarrow> 'a \<Rightarrow> 'sugar " (
 translations " (a \<tycolon> A) \<heavy_asterisk> (b \<tycolon> B) " \<rightleftharpoons> " (CONST Pair b a) \<tycolon> (B <heap-sep> A) "
   " A \<heavy_asterisk> B " => " (CONST Pair (_\<nu>typing_x B) (_\<nu>typing_x A)) \<tycolon> ((_\<nu>typing_ty B) <heap-sep> (_\<nu>typing_ty A)) "
 
+lemma Heap_Delimiter_cong: "\<tort_lbrace>h1 \<tycolon> H1\<tort_rbrace> \<equiv> \<tort_lbrace>h1' \<tycolon> H1'\<tort_rbrace> \<Longrightarrow> \<tort_lbrace>h2 \<tycolon> H2\<tort_rbrace> \<equiv> \<tort_lbrace>h2' \<tycolon> H2'\<tort_rbrace> \<Longrightarrow> \<tort_lbrace>h1 \<tycolon> H1 \<heavy_asterisk> h2 \<tycolon> H2\<tort_rbrace> \<equiv> \<tort_lbrace>h1' \<tycolon> H1' \<heavy_asterisk> h2' \<tycolon> H2'\<tort_rbrace>"
+  unfolding atomize_eq Heap_Delimiter_def by (auto 0 5 simp add: nu_exps)
+simproc_setup Heap_Delimiter_cong ("\<tort_lbrace>h1 \<tycolon> H1 \<heavy_asterisk> h2 \<tycolon> H2\<tort_rbrace>") = \<open>K (NuSimpCong.simproc @{thm Heap_Delimiter_cong})\<close>
 
 
 
@@ -507,6 +515,8 @@ translations " a \<tycolon> A\<heavy_comma> b \<tycolon> B " == " (CONST Pair b 
 
 lemma [nu_exps]: "(pa,pb) \<nuLinkL> A <stack-div> B \<nuLinkR> (xa,xb) \<longleftrightarrow> (pa \<nuLinkL> A \<nuLinkR> xa) \<and> (pb \<nuLinkL> B \<nuLinkR> xb)"
   unfolding Stack_Delimiter_def by (simp add: nu_exps)
+lemma [\<nu>elim,elim!]: "(a,b) \<ratio> A <stack-div> B \<Longrightarrow> (a \<ratio> A \<Longrightarrow> b \<ratio> B \<Longrightarrow> C) \<Longrightarrow> C"
+  unfolding Stack_Delimiter_def by blast
 
 lemma [\<nu>intro]: "\<^bold>c\<^bold>a\<^bold>s\<^bold>t a \<tycolon> A \<longmapsto> a' \<tycolon> A' \<^bold>w\<^bold>i\<^bold>t\<^bold>h P1 \<Longrightarrow> (P1 \<Longrightarrow> \<^bold>c\<^bold>a\<^bold>s\<^bold>t b \<tycolon> B \<longmapsto> b' \<tycolon> B' \<^bold>w\<^bold>i\<^bold>t\<^bold>h P2) \<Longrightarrow>
   \<^bold>c\<^bold>a\<^bold>s\<^bold>t (a \<tycolon> A\<heavy_comma> b \<tycolon> B) \<longmapsto> (a' \<tycolon> A'\<heavy_comma> b' \<tycolon> B') \<^bold>w\<^bold>i\<^bold>t\<^bold>h P1 \<and> P2"
@@ -566,10 +576,10 @@ syntax "_ExNu_print" :: "logic \<Rightarrow> logic \<Rightarrow> logic"
 
 translations "\<exists>* a b. P" \<rightleftharpoons> "\<exists>* a. (\<exists>*b. P)"
   "\<exists>* c. x \<tycolon> T" => "(\<lambda>c. x) \<tycolon> CONST ExNu (\<lambda>c. T)"
-  "\<exists>* c. x \<tycolon> T" <= "(\<lambda>c. x) \<tycolon> CONST ExNu (\<lambda>c''''''. T)" (*TODO: print translation that alpha-convert the c''''' *)
+(*  "\<exists>* c. x \<tycolon> T" <= "(\<lambda>c. x) \<tycolon> CONST ExNu (\<lambda>c''''''. T)" (*TODO: print translation that alpha-convert the c''''' *)
   "\<exists>* c. x c \<tycolon> T" <= "x \<tycolon> CONST ExNu (\<lambda>c. T)"
   "CONST Pair a b" <= "(CONST Pair a) b"
-  "\<exists>* c. x \<tycolon> T c" <= "(\<lambda>c. x) \<tycolon> CONST ExNu T"
+  "\<exists>* c. x \<tycolon> T c" <= "(\<lambda>c. x) \<tycolon> CONST ExNu T" *)
 
 notation ExNu_sugar (binder "\<exists>\<^sup>\<nu> " 10)
 
@@ -633,6 +643,11 @@ lemma [simp]: "p \<nuLinkL> T \<and>\<^sup>\<nu> P \<nuLinkR> x \<longleftrighta
 
 lemma [\<nu>intro]: "\<^bold>p\<^bold>r\<^bold>e\<^bold>m\<^bold>i\<^bold>s\<^bold>e P \<Longrightarrow> \<^bold>i\<^bold>n\<^bold>t\<^bold>r\<^bold>o \<^bold>c\<^bold>a\<^bold>s\<^bold>t x \<tycolon> T \<longmapsto> (x \<tycolon> T) \<and>\<^sup>\<nu> P"
   unfolding Intro_def Cast_def Premise_def by (simp add: nu_exps)
+lemma [\<nu>intro]: "\<^bold>c\<^bold>a\<^bold>s\<^bold>t x \<tycolon> T \<longmapsto> x' \<tycolon> T' \<^bold>w\<^bold>i\<^bold>t\<^bold>h P \<Longrightarrow> \<^bold>p\<^bold>r\<^bold>e\<^bold>m\<^bold>i\<^bold>s\<^bold>e (P \<longrightarrow> Q) \<Longrightarrow> \<^bold>c\<^bold>a\<^bold>s\<^bold>t x \<tycolon> T \<longmapsto> x' \<tycolon> T' \<and>\<^sup>\<nu> Q \<^bold>w\<^bold>i\<^bold>t\<^bold>h P"
+  unfolding Cast_def Premise_def by (simp add: nu_exps)
+
+lemma subj_\<nu>app: "\<^bold>p\<^bold>a\<^bold>r\<^bold>a\<^bold>m P \<Longrightarrow> \<^bold>p\<^bold>r\<^bold>e\<^bold>m\<^bold>i\<^bold>s\<^bold>e P \<Longrightarrow> \<^bold>c\<^bold>a\<^bold>s\<^bold>t x \<tycolon> N \<longmapsto> x \<tycolon> N \<and>\<^sup>\<nu> P"
+  unfolding Cast_def Premise_def by simp
 
 (* lemma [simp]: "\<tort_lbrace> x \<tycolon> T \<and>\<^sup>\<nu> True\<tort_rbrace> = \<tort_lbrace> x \<tycolon> T \<tort_rbrace>" by auto
 lemma [simp]: "\<tort_lbrace>L \<heavy_comma> (x \<tycolon> T) \<and> P\<tort_rbrace> = \<tort_lbrace>(L \<heavy_comma> x \<tycolon> T) \<and> P\<tort_rbrace>" and [simp]: "\<tort_lbrace>(x \<tycolon> T) \<and> P\<heavy_comma> R\<tort_rbrace> = \<tort_lbrace>(x \<tycolon> T\<heavy_comma> R) \<and> P\<tort_rbrace>"
@@ -641,22 +656,6 @@ lemma [simp]: "\<tort_lbrace>L \<heavy_asterisk> (x \<tycolon> T) \<and> P\<tort
   unfolding Heap_Delimiter_def by auto blast+
 lemma [simp]: "\<tort_lbrace> (s \<tycolon> S) \<and> P \<heavy_comma> \<^bold>h\<^bold>e\<^bold>a\<^bold>p h \<tycolon> H \<tort_rbrace> = \<tort_lbrace> (s \<tycolon> S\<heavy_comma> \<^bold>h\<^bold>e\<^bold>a\<^bold>p h \<tycolon> H) \<and> P \<tort_rbrace>"
   and [simp]: "\<tort_lbrace> s \<tycolon> S \<heavy_comma> \<^bold>h\<^bold>e\<^bold>a\<^bold>p (h \<tycolon> H) \<and> P \<tort_rbrace> = \<tort_lbrace> (s \<tycolon> S\<heavy_comma> \<^bold>h\<^bold>e\<^bold>a\<^bold>p h \<tycolon> H) \<and> P \<tort_rbrace>" by auto *)
-
-
-lemma t1: "(\<^bold>c\<^bold>u\<^bold>r\<^bold>r\<^bold>e\<^bold>n\<^bold>t s \<^bold>r\<^bold>e\<^bold>s\<^bold>u\<^bold>l\<^bold>t\<^bold>s \<^bold>i\<^bold>n (x \<tycolon> T) \<and> P) \<longleftrightarrow> (\<^bold>c\<^bold>u\<^bold>r\<^bold>r\<^bold>e\<^bold>n\<^bold>t s \<^bold>r\<^bold>e\<^bold>s\<^bold>u\<^bold>l\<^bold>t\<^bold>s \<^bold>i\<^bold>n x \<tycolon> T) \<and> P"
-  unfolding CurrentConstruction_def by (cases s) (simp add: nu_exps, blast+)
-lemma [simp]: "((((\<^bold>c\<^bold>u\<^bold>r\<^bold>r\<^bold>e\<^bold>n\<^bold>t s \<^bold>r\<^bold>e\<^bold>s\<^bold>u\<^bold>l\<^bold>t\<^bold>s \<^bold>i\<^bold>n T) \<and> B) \<and> C) \<^bold>w\<^bold>i\<^bold>t\<^bold>h \<^bold>f\<^bold>a\<^bold>c\<^bold>t\<^bold>s: PROP L) \<equiv> (((\<^bold>c\<^bold>u\<^bold>r\<^bold>r\<^bold>e\<^bold>n\<^bold>t s \<^bold>r\<^bold>e\<^bold>s\<^bold>u\<^bold>l\<^bold>t\<^bold>s \<^bold>i\<^bold>n T) \<and> (B \<and> C)) \<^bold>w\<^bold>i\<^bold>t\<^bold>h \<^bold>f\<^bold>a\<^bold>c\<^bold>t\<^bold>s: PROP L)" by simp
-
-lemma move_fact_to_star1[simp]:
-  "((\<^bold>c\<^bold>u\<^bold>r\<^bold>r\<^bold>e\<^bold>n\<^bold>t s \<^bold>r\<^bold>e\<^bold>s\<^bold>u\<^bold>l\<^bold>t\<^bold>s \<^bold>i\<^bold>n (x \<tycolon> T) \<and> Q) \<^bold>w\<^bold>i\<^bold>t\<^bold>h \<^bold>f\<^bold>a\<^bold>c\<^bold>t\<^bold>s: PROP FactCollection (PROP NoFact) (PROP L) (PROP I))
-    \<Longrightarrow> (\<^bold>c\<^bold>u\<^bold>r\<^bold>r\<^bold>e\<^bold>n\<^bold>t s \<^bold>r\<^bold>e\<^bold>s\<^bold>u\<^bold>l\<^bold>t\<^bold>s \<^bold>i\<^bold>n x \<tycolon> T \<^bold>w\<^bold>i\<^bold>t\<^bold>h \<^bold>f\<^bold>a\<^bold>c\<^bold>t\<^bold>s: PROP FactCollection (Trueprop Q) (PROP L) (PROP I))"
-  unfolding t1 SpecTop_imp conj_imp FactCollection_imp
-  by (intro equal_intr_rule SpecTop_I FactCollection_I conjI NoFact) (* (unfold SpecTop_imp conj_imp FactCollection_imp) *)
-lemma move_fact_to_star2[simp]:
-  "((\<^bold>c\<^bold>u\<^bold>r\<^bold>r\<^bold>e\<^bold>n\<^bold>t s \<^bold>r\<^bold>e\<^bold>s\<^bold>u\<^bold>l\<^bold>t\<^bold>s \<^bold>i\<^bold>n (x \<tycolon> T) \<and> Q) \<^bold>w\<^bold>i\<^bold>t\<^bold>h \<^bold>f\<^bold>a\<^bold>c\<^bold>t\<^bold>s: PROP FactCollection (Trueprop P) (PROP L) (PROP I))
-    \<Longrightarrow> (\<^bold>c\<^bold>u\<^bold>r\<^bold>r\<^bold>e\<^bold>n\<^bold>t s \<^bold>r\<^bold>e\<^bold>s\<^bold>u\<^bold>l\<^bold>t\<^bold>s \<^bold>i\<^bold>n x \<tycolon> T \<^bold>w\<^bold>i\<^bold>t\<^bold>h \<^bold>f\<^bold>a\<^bold>c\<^bold>t\<^bold>s: PROP FactCollection  (Trueprop (Q \<and> P)) (PROP L) (PROP I))"
-  unfolding t1 SpecTop_imp conj_imp FactCollection_imp
-  by (intro equal_intr_rule SpecTop_I FactCollection_I conjI) (* (unfold SpecTop_imp conj_imp FactCollection_imp) *)
 
 lemma NuAddition_cong: "\<tort_lbrace>x \<tycolon> T\<tort_rbrace> \<equiv> \<tort_lbrace>x' \<tycolon> T'\<tort_rbrace> \<Longrightarrow> \<tort_lbrace>x \<tycolon> T \<and>\<^sup>\<nu> P\<tort_rbrace> \<equiv> \<tort_lbrace>x' \<tycolon> T' \<and>\<^sup>\<nu> P\<tort_rbrace>" unfolding atomize_eq by (auto simp add: nu_exps)
 simproc_setup NuAddition_cong ("\<tort_lbrace>x \<tycolon> T \<and>\<^sup>\<nu> P\<tort_rbrace>") = \<open>K (NuSimpCong.simproc @{thm NuAddition_cong})\<close>
@@ -693,6 +692,22 @@ lemma [simp]: "\<tort_lbrace>c \<tycolon> Ctx \<and>\<^sup>\<nu>\<^sub>a\<^sub>u
 lemma AutoAddition_cong: "\<tort_lbrace>x \<tycolon> T\<tort_rbrace> \<equiv> \<tort_lbrace>x' \<tycolon> T'\<tort_rbrace> \<Longrightarrow> \<tort_lbrace>x \<tycolon> T \<and>\<^sup>\<nu>\<^sub>a\<^sub>u\<^sub>t\<^sub>o P\<tort_rbrace> \<equiv> \<tort_lbrace>x' \<tycolon> T' \<and>\<^sup>\<nu>\<^sub>a\<^sub>u\<^sub>t\<^sub>o P\<tort_rbrace>" unfolding Auto_def by simp
 simproc_setup AutoAddition_cong ("\<tort_lbrace>x \<tycolon> T \<and>\<^sup>\<nu>\<^sub>a\<^sub>u\<^sub>t\<^sub>o P\<tort_rbrace>") = \<open>K (NuSimpCong.simproc @{thm AutoAddition_cong})\<close>
 
+lemma t1: "(\<^bold>c\<^bold>u\<^bold>r\<^bold>r\<^bold>e\<^bold>n\<^bold>t s \<^bold>r\<^bold>e\<^bold>s\<^bold>u\<^bold>l\<^bold>t\<^bold>s \<^bold>i\<^bold>n (x \<tycolon> T) \<and>\<^sup>\<nu>\<^sub>a\<^sub>u\<^sub>t\<^sub>o P) \<longleftrightarrow> (\<^bold>c\<^bold>u\<^bold>r\<^bold>r\<^bold>e\<^bold>n\<^bold>t s \<^bold>r\<^bold>e\<^bold>s\<^bold>u\<^bold>l\<^bold>t\<^bold>s \<^bold>i\<^bold>n x \<tycolon> T) \<and> P"
+  unfolding CurrentConstruction_def Auto_def by (cases s) (simp add: nu_exps, blast+)
+lemma [simp]: "((((\<^bold>c\<^bold>u\<^bold>r\<^bold>r\<^bold>e\<^bold>n\<^bold>t s \<^bold>r\<^bold>e\<^bold>s\<^bold>u\<^bold>l\<^bold>t\<^bold>s \<^bold>i\<^bold>n T) \<and> B) \<and> C) \<^bold>w\<^bold>i\<^bold>t\<^bold>h \<^bold>f\<^bold>a\<^bold>c\<^bold>t\<^bold>s: PROP L) \<equiv> (((\<^bold>c\<^bold>u\<^bold>r\<^bold>r\<^bold>e\<^bold>n\<^bold>t s \<^bold>r\<^bold>e\<^bold>s\<^bold>u\<^bold>l\<^bold>t\<^bold>s \<^bold>i\<^bold>n T) \<and> (B \<and> C)) \<^bold>w\<^bold>i\<^bold>t\<^bold>h \<^bold>f\<^bold>a\<^bold>c\<^bold>t\<^bold>s: PROP L)" by simp
+
+lemma move_fact_to_star1[simp]:
+  "((\<^bold>c\<^bold>u\<^bold>r\<^bold>r\<^bold>e\<^bold>n\<^bold>t s \<^bold>r\<^bold>e\<^bold>s\<^bold>u\<^bold>l\<^bold>t\<^bold>s \<^bold>i\<^bold>n (x \<tycolon> T) \<and>\<^sup>\<nu>\<^sub>a\<^sub>u\<^sub>t\<^sub>o Q) \<^bold>w\<^bold>i\<^bold>t\<^bold>h \<^bold>f\<^bold>a\<^bold>c\<^bold>t\<^bold>s: PROP FactCollection (PROP NoFact) (PROP L) (PROP I))
+    \<Longrightarrow> (\<^bold>c\<^bold>u\<^bold>r\<^bold>r\<^bold>e\<^bold>n\<^bold>t s \<^bold>r\<^bold>e\<^bold>s\<^bold>u\<^bold>l\<^bold>t\<^bold>s \<^bold>i\<^bold>n x \<tycolon> T \<^bold>w\<^bold>i\<^bold>t\<^bold>h \<^bold>f\<^bold>a\<^bold>c\<^bold>t\<^bold>s: PROP FactCollection (Trueprop Q) (PROP L) (PROP I))"
+  unfolding t1 SpecTop_imp conj_imp FactCollection_imp
+  by (intro equal_intr_rule SpecTop_I FactCollection_I conjI NoFact) (* (unfold SpecTop_imp conj_imp FactCollection_imp) *)
+lemma move_fact_to_star2[simp]:
+  "((\<^bold>c\<^bold>u\<^bold>r\<^bold>r\<^bold>e\<^bold>n\<^bold>t s \<^bold>r\<^bold>e\<^bold>s\<^bold>u\<^bold>l\<^bold>t\<^bold>s \<^bold>i\<^bold>n (x \<tycolon> T) \<and>\<^sup>\<nu>\<^sub>a\<^sub>u\<^sub>t\<^sub>o Q) \<^bold>w\<^bold>i\<^bold>t\<^bold>h \<^bold>f\<^bold>a\<^bold>c\<^bold>t\<^bold>s: PROP FactCollection (Trueprop P) (PROP L) (PROP I))
+    \<Longrightarrow> (\<^bold>c\<^bold>u\<^bold>r\<^bold>r\<^bold>e\<^bold>n\<^bold>t s \<^bold>r\<^bold>e\<^bold>s\<^bold>u\<^bold>l\<^bold>t\<^bold>s \<^bold>i\<^bold>n x \<tycolon> T \<^bold>w\<^bold>i\<^bold>t\<^bold>h \<^bold>f\<^bold>a\<^bold>c\<^bold>t\<^bold>s: PROP FactCollection  (Trueprop (Q \<and> P)) (PROP L) (PROP I))"
+  unfolding t1 SpecTop_imp conj_imp FactCollection_imp
+  by (intro equal_intr_rule SpecTop_I FactCollection_I conjI) (* (unfold SpecTop_imp conj_imp FactCollection_imp) *)
+
+
 subsection \<open>Identity\<close>
 
 definition Identity :: " ('a::lrep, 'a) \<nu> " where "Identity x = {x}"
@@ -718,7 +733,7 @@ lemma refine_\<nu>app: "\<^bold>p\<^bold>a\<^bold>r\<^bold>a\<^bold>m P \<Longri
   unfolding Cast_def by (simp add: nu_exps) blast
 
 abbreviation AutoRefine (infixl "<auto-where>" 80)
-  where "AutoRefine \<equiv> Auto NuRefine"
+  where "AutoRefine N P \<equiv> Auto (NuRefine N P)"
 lemma [simp]:"\<tort_lbrace>x \<tycolon> T <auto-where> P \<tort_rbrace> = \<tort_lbrace> (x \<tycolon> T) \<and>\<^sup>\<nu>\<^sub>a\<^sub>u\<^sub>t\<^sub>o (\<^bold>p\<^bold>r\<^bold>e\<^bold>m\<^bold>i\<^bold>s\<^bold>e x \<in> P) \<tort_rbrace>"
   unfolding Auto_def Premise_def by (auto simp add: nu_exps)
 
@@ -832,6 +847,20 @@ lemma "\<^bold>c\<^bold>a\<^bold>s\<^bold>t x \<tycolon> N \<longmapsto> f x \<t
 
 lemma "\<nu>Equal (N <up-lift> f) can_eq eq \<longleftrightarrow> \<nu>Equal N (inv_imagep can_eq f) (inv_imagep eq f)"
   unfolding \<nu>Equal_def by (auto 0 6)
+
+
+subsubsection \<open>Operator Some\<close>
+
+definition NuSome :: " ('a :: lrep, 'b) \<nu> \<Rightarrow> ('a :: lrep, 'b set) \<nu> " ("<some>")
+  where "NuSome T S = {p. (\<exists>x. x \<in> S \<and> (p \<nuLinkL> T \<nuLinkR> x)) }"
+notation NuSome ("\<^bold>s\<^bold>o\<^bold>m\<^bold>e")
+
+lemma [simp]: "p \<nuLinkL> \<^bold>s\<^bold>o\<^bold>m\<^bold>e T \<nuLinkR> X \<longleftrightarrow> (\<exists>x. x \<in> X \<and> (p \<nuLinkL>T \<nuLinkR> x))" unfolding NuSome_def Refining_def by simp
+lemma [elim,\<nu>elim]: "X \<ratio> (\<^bold>s\<^bold>o\<^bold>m\<^bold>e T) \<Longrightarrow> (\<And>x. x \<in> X \<Longrightarrow> x \<ratio> T \<Longrightarrow> C) \<Longrightarrow> C" unfolding Inhabited_def by simp blast
+(* lemma [\<nu>intro]: "\<^bold>p\<^bold>r\<^bold>e\<^bold>m\<^bold>i\<^bold>s\<^bold>e X \<subseteq> X' \<Longrightarrow> [h] \<^bold>c\<^bold>a\<^bold>s\<^bold>t X \<tycolon> (\<^bold>s\<^bold>o\<^bold>m\<^bold>e N) \<longmapsto> X' \<tycolon> (\<^bold>s\<^bold>o\<^bold>m\<^bold>e N)" unfolding Cast_def by (auto 2 3) *)
+lemma [\<nu>intro]: "\<^bold>c\<^bold>a\<^bold>s\<^bold>t x \<tycolon> N \<longmapsto> y \<tycolon> M \<^bold>w\<^bold>i\<^bold>t\<^bold>h P \<Longrightarrow> \<^bold>p\<^bold>r\<^bold>e\<^bold>m\<^bold>i\<^bold>s\<^bold>e y \<in> Y \<Longrightarrow> \<^bold>c\<^bold>a\<^bold>s\<^bold>t x \<tycolon> N \<longmapsto> Y \<tycolon> (\<^bold>s\<^bold>o\<^bold>m\<^bold>e M) \<^bold>w\<^bold>i\<^bold>t\<^bold>h P" unfolding Cast_def by auto
+(*lemma someI_\<nu>cast: "\<^bold>p\<^bold>a\<^bold>r\<^bold>a\<^bold>m X \<Longrightarrow> \<^bold>p\<^bold>r\<^bold>e\<^bold>m\<^bold>i\<^bold>s\<^bold>e x \<in> X \<Longrightarrow> [h] \<^bold>c\<^bold>a\<^bold>s\<^bold>t x \<tycolon> N \<longmapsto> X \<tycolon> (\<^bold>s\<^bold>o\<^bold>m\<^bold>e N)" unfolding Cast_def by auto
+lemma someE_\<nu>cast[\<nu>cast_overload E]: "[h] \<^bold>c\<^bold>a\<^bold>s\<^bold>t X \<tycolon> (\<^bold>s\<^bold>o\<^bold>m\<^bold>e N) \<longmapsto> (\<exists>*some. \<tort_lbrace>some \<tycolon> N \<tort_rbrace> \<addition> (some \<in> X))" unfolding Cast_def by auto *)
 
 
 section \<open>Mechanisms - II\<close>
@@ -1144,7 +1173,7 @@ lemma op_call:
   unfolding Procedure_def Function_def op_call_def Arguments_def
   by (cases args, cases rets) (auto 0 5 simp add: pair_forall split: state.split prod.split)
 
-lemma rename_func: "f \<equiv> f' \<Longrightarrow> \<^bold>f\<^bold>u\<^bold>n\<^bold>c f' \<blangle> U \<longmapsto> \<R> \<brangle> \<Longrightarrow> \<^bold>f\<^bold>u\<^bold>n\<^bold>c f \<blangle> U \<longmapsto> \<R> \<brangle>" by fast
+lemma rename_func: "f \<equiv> f' \<Longrightarrow> \<^bold>f\<^bold>u\<^bold>n\<^bold>c f' \<blangle> U \<longmapsto> \<R> \<brangle> \<Longrightarrow> \<^bold>f\<^bold>u\<^bold>n\<^bold>c f \<blangle> U \<longmapsto> \<R> \<brangle>" by blast
 
 subsubsection \<open>Recursive Function\<close>
 
@@ -1506,8 +1535,8 @@ declare
   "cast"[OF _ cast_whole_heap_\<nu>app[OF Argument_I, OF cast_heap_conversion],
       \<nu>application_method 2 20]
 
-lemmas apply_func[\<nu>application_method 3 70] = apply_proc[OF _ op_call]
-lemmas apply_func_conv[\<nu>application_method 3 -2000] = apply_proc_conv[OF _ _ op_call, rotated 1 1]
+(*lemmas apply_func[\<nu>application_method 3 70] = apply_proc[OF _ op_call]*)
+lemmas apply_func_conv[\<nu>application_method 3 100] = apply_proc_conv[OF _ _ op_call, rotated 1 1]
 
 (* consts \<nu>Application_Rewrite :: bool
 setup_\<nu>application_method \<open>\<nu>Application_Rewrite\<close> 1000 \<open>PROP P &&& A = B\<close> | \<open>PROP P &&& (A \<equiv> B)\<close> = \<open>
@@ -1552,7 +1581,7 @@ subsection \<open>Constructive\<close>
 
 \<nu>processor accept_proc 300 \<open>\<^bold>p\<^bold>e\<^bold>n\<^bold>d\<^bold>i\<^bold>n\<^bold>g f \<^bold>o\<^bold>n blk \<^bold>r\<^bold>e\<^bold>s\<^bold>u\<^bold>l\<^bold>t\<^bold>s \<^bold>i\<^bold>n T\<close> \<open>fn ctx => fn th => Scan.succeed (fn _ => NuSys.accept_proc ctx th)\<close>
 
-\<nu>processor move_fact 50 \<open>(\<^bold>c\<^bold>u\<^bold>r\<^bold>r\<^bold>e\<^bold>n\<^bold>t blk \<^bold>r\<^bold>e\<^bold>s\<^bold>u\<^bold>l\<^bold>t\<^bold>s \<^bold>i\<^bold>n (x \<tycolon> T) \<and> P)\<close> \<open>fn ctx => fn meta => Scan.succeed (fn _ =>
+\<nu>processor move_fact 50 \<open>(\<^bold>c\<^bold>u\<^bold>r\<^bold>r\<^bold>e\<^bold>n\<^bold>t blk \<^bold>r\<^bold>e\<^bold>s\<^bold>u\<^bold>l\<^bold>t\<^bold>s \<^bold>i\<^bold>n (x \<tycolon> T) \<and>\<^sup>\<nu>\<^sub>a\<^sub>u\<^sub>t\<^sub>o P)\<close> \<open>fn ctx => fn meta => Scan.succeed (fn _ =>
   meta RS @{thm move_fact_to_star1} handle THM _ => meta RS @{thm move_fact_to_star2})\<close>
 
 \<nu>processor "apply" 9000 \<open>P\<close> \<open> fn ctx => fn meta => NuApplicant.parser >> (fn binding => fn _ =>
@@ -1677,22 +1706,22 @@ lemma Variants_Subj_I: "Variants_Subj vars subj" unfolding Variants_Subj_def .. 
 lemma case_prod_expn_I: "A = B x y \<Longrightarrow> A = case_prod B (x,y)" by simp
 lemma case_named_expn_I: "A = B x \<Longrightarrow> A = case_named B (tag x)" by simp
 
-ML_file \<open>library/variables_tag.ML\<close>
+ML_file_debug \<open>library/variables_tag.ML\<close>
 
 \<nu>processor vars_by_pattern 110 \<open>Variant_Cast (s \<tycolon> S) (h \<tycolon> H) vars S' H' \<Longrightarrow> PROP P\<close> \<open>fn ctx => fn meta => 
 let open Parse Scan NuHelp NuBasics in
+  ($$$ "var" |-- list1 params -- option ($$$ "in" |-- list1 term) -- option ($$$ "heap" |-- list1 term) -- Scan.option ($$$ "always" |-- term))
+    >> (fn ((((vars, stack_schema), heap_schema)), always) => fn _ =>
+      NuVariablesTag.variables_tag_pattern_match (flat vars) stack_schema heap_schema always ctx meta |> @{print})
+||
   (list1 term -- Scan.option ($$$ "always" |-- term) >> (fn (vars, always) => fn _ =>
       NuVariablesTag.variables_tag_terms vars always ctx meta) )
-||
-  (list1 params -- option ($$$ "in" |-- list1 term) -- option ($$$ "heap" |-- list1 term) -- Scan.option ($$$ "always" |-- term))
-    >> (fn ((((vars, stack_schema), heap_schema)), always) => fn _ =>
-      NuVariablesTag.variables_tag_pattern_match (flat vars) stack_schema heap_schema always ctx meta)
 end\<close>
 
 subsection \<open>Auto Reasoners\<close>
 
 ML_file "library/reasoners.ML"
 
-\<nu>reasoner \<open>\<^bold>p\<^bold>r\<^bold>e\<^bold>m\<^bold>i\<^bold>s\<^bold>e P\<close> 0 = \<open>Nu_Reasoners.premise_tac\<close>
+\<nu>reasoner \<open>\<^bold>p\<^bold>r\<^bold>e\<^bold>m\<^bold>i\<^bold>s\<^bold>e P\<close> 10 = \<open>Nu_Reasoners.premise_tac\<close>
 
 end
