NuPrime.thy
@@ -321,7 +321,7 @@ definition Premise :: "bool \<Rightarrow> bool" ("\<^bold>p\<^bold>r\<^bold>e\<^
   \<comment> \<open>The tag represent a necessary premise that must be solved in a rule or procedure.
     The automatic reasoning ties to solve it, and if fails, terminates the automatic reasoning.\<close>
 
-lemma Premise_I: "P \<Longrightarrow> \<^bold>p\<^bold>r\<^bold>e\<^bold>m\<^bold>i\<^bold>s\<^bold>e P" unfolding Premise_def by simp
+lemma Premise_I[intro!]: "P \<Longrightarrow> \<^bold>p\<^bold>r\<^bold>e\<^bold>m\<^bold>i\<^bold>s\<^bold>e P" unfolding Premise_def by simp
 lemma Premise_E: "\<^bold>p\<^bold>r\<^bold>e\<^bold>m\<^bold>i\<^bold>s\<^bold>e P \<Longrightarrow> P" unfolding Premise_def by simp
 
 lemma [elim!,\<nu>elim]: "\<^bold>p\<^bold>r\<^bold>e\<^bold>m\<^bold>i\<^bold>s\<^bold>e P \<Longrightarrow> (P \<Longrightarrow> C) \<Longrightarrow> C" unfolding Premise_def by simp
